src/high/resources/auth_map_map.v
@@ -1,6 +1,7 @@
 From iris.algebra Require Import auth gmap.
 From iris.base_logic.lib Require Import own.
 From iris.proofmode Require Import proofmode.
+From iris_named_props Require Import named_props.
 
 From self.lang Require Import lang.
 From self Require Import extra.
@@ -8,118 +9,36 @@ From self Require Import extra.
 From self.nextgen Require Import hvec nextgen_promises.
 From self.base Require Import generational_resources.
 
+Set Default Proof Using "Type*".
 
-Definition auth_map_mapR (A : ofe) :=
-  authR (gmapUR loc (gmapUR time (agreeR A))).
-
-Definition fmap_fmap_to_agree_ol (m : gmap loc (gmap time positive)) : gmapUR loc _ :=
-  (λ n : gmap _ _, to_agree <$> n) <$> m.
-
-Section fmap_fmap_to_agree.
-  Context {A : ofe}.
-  Implicit Types (m : gmap loc (gmap time A)).
-
-  Definition fmap_fmap_to_agree m : gmap loc (gmap time (agreeR A)) :=
-    (λ n : gmap _ _, (to_agree) <$> n) <$> m.
-
-  Lemma fmap_fmap_to_agree_valid m : ✓ fmap_fmap_to_agree m.
-  Proof.
-    rewrite /fmap_fmap_to_agree.
-    intros ?.
-    rewrite lookup_fmap.
-    destruct (m !! i); last done.
-    simpl.
-    apply Some_valid.
-    apply valid_to_agree_fmap.
-  Qed.
-
-  Lemma fmap_fmap_to_agree_mono m1 m2 :
-    m1 ⊆ m2 → fmap_fmap_to_agree m1 ≼ fmap_fmap_to_agree m2.
-  Proof.
-    rewrite map_subseteq_spec.
-    intros sub.
-    rewrite /fmap_fmap_to_agree.
-    rewrite lookup_included.
-    setoid_rewrite lookup_fmap.
-    intros i.
-    destruct (m1 !! i) eqn:eq.
-    2: { eexists _. rewrite left_id. reflexivity. }
-    rewrite (sub i g); last done.
-    done.
-  Qed.
-
-  Lemma fmap_fmap_to_agree_singleton_included_l `{!LeibnizEquiv A}
-        m (i : loc) (x : gmap time A) :
-    fmap_fmap_to_agree {[ i := x ]} ≼ fmap_fmap_to_agree m →
-    (∃ (y : gmap _ _), m !! i ≡ Some y ∧ x ⊆ y).
-  Proof.
-    rewrite /fmap_fmap_to_agree.
-    rewrite map_fmap_singleton.
-    rewrite singleton_included_l.
-    rewrite lookup_fmap.
-    intros [agh [equiv incl]].
-    apply fmap_Some_equiv in equiv as [h [look equiv]].
-    exists h.
-    split; first by rewrite look. 
-    move: incl.
-    rewrite Some_included_total.
-    rewrite equiv.
-    rewrite -to_agree_fmap. done.
-  Qed.
-
-  Lemma fmap_fmap_to_agree_incl `{!LeibnizEquiv A} m m' :
-    dom m ⊆ dom m' →
-    (∀ ℓ mi mi', m !! ℓ = Some mi → m' !! ℓ = Some mi' → mi ⊆ mi') →
-    (fmap_fmap_to_agree m) ≼ (fmap_fmap_to_agree m').
-  Proof.
-    intros subOut subIn.
-    rewrite /fmap_fmap_to_agree.
-    apply lookup_included => ℓ.
-    rewrite 2!lookup_fmap.
-    destruct (m !! ℓ) as [mi|] eqn:lookM.
-    2: { apply option_included. naive_solver. }
-    destruct (m' !! ℓ) as [mi'|] eqn:lookM'.
-    2: { exfalso.
-         apply not_elem_of_dom in lookM'.
-         apply elem_of_dom_2 in lookM.
-         set_solver. }
-    simpl.
-    apply Some_included_total.
-    apply to_agree_fmap.
-    eapply subIn; done.
-  Qed.
-
-  Lemma fmap_fmap_to_agree_singleton ℓ h :
-    fmap_fmap_to_agree {[ℓ := h]} = {[ℓ := to_agree <$> h]}.
-  Proof. by rewrite /fmap_fmap_to_agree map_fmap_singleton. Qed.
-
-End fmap_fmap_to_agree.
+Definition auth_map_mapR (A: ofe) :=
+  authR (gmapUR (loc * time) (agreeR A)).
 
 Section auth_map_map.
   Context {A : ofe}.
   Notation auth_map_mapR_inG Σ Ω := (genInDepsG Σ Ω (auth_map_mapR A) [#crashed_atR]).
-  Context `{!nvmBaseGS Σ Ω, !auth_map_mapR_inG Σ Ω}.
+  Context `{!nvmBaseGS Σ Ω, inG: !auth_map_mapR_inG Σ Ω}.
 
+  Variable (R: rel_over [#crashed_atR] (auth_map_mapR A)).
   Implicit Types (m : gmap loc (gmap time A)).
 
-  Definition auth_map_map_auth γ m :=
-    gen_own γ (● (fmap_fmap_to_agree m)).
+  Definition agree_uncurry_map m: gmap (loc * time) (agreeR A) := to_agree <$> (gmap_uncurry m).
+  
+  Definition auth_map_map_auth γ m: iProp Σ :=
+    "own_auth" ∷ gen_own γ (● agree_uncurry_map m) ∗
+    "#rely" ∷ rely (g := inG) γ [#crashed_at_name] R True_pred ∗
+    "#crashed" ∷ ∃ OCV, crashed_at_offset OCV.
 
-  Definition auth_map_map_auth_dq γ dq m :=
-    gen_own γ (●{dq} (fmap_fmap_to_agree m)).
-
-  Definition auth_map_map_frag γ m :=
-    gen_own γ (◯ (fmap_fmap_to_agree m)).
-
-  Definition auth_map_map_frag_singleton γ ℓ t a :=
-    auth_map_map_frag γ {[ ℓ := {[ t := a ]} ]}.
+  Definition auth_map_map_frag_singleton γ ℓ t a: iProp Σ :=
+    "own_frag" ∷ gen_own γ (◯ {[ (ℓ, t) := to_agree a ]}) ∗
+    "#rely" ∷ rely (g := inG) γ [#crashed_at_name] R True_pred ∗
+    "#crashed" ∷ ∃ OCV, crashed_at_offset OCV.
 
   (* TODO: allocation lemma *)
-
-  Lemma auth_map_map_alloc m :
-    ⊢ |==> ∃ γ, auth_map_map_auth γ m ∗ auth_map_map_frag γ m.
-  Proof.
-  Admitted.
+  (* Lemma auth_map_map_alloc m : *)
+  (*   ⊢ |==> ∃ γ, auth_map_map_auth γ m ∗ auth_map_map_frag γ m. *)
+  (* Proof. *)
+  (* Admitted. *)
 
   Lemma auth_map_map_lookup `{!LeibnizEquiv A} γ m ℓ t h a :
     m !! ℓ = Some h →
@@ -127,36 +46,68 @@ Section auth_map_map.
     auth_map_map_auth γ m ==∗
     auth_map_map_auth γ m ∗ auth_map_map_frag_singleton γ ℓ t a.
   Proof.
-    iIntros (mLook hLook) "N".
-    rewrite /auth_map_map_auth /auth_map_map_frag. setoid_rewrite <- own_op.
+    iIntros (mLook hLook) "(N & #$ & #$)".
+    rewrite /auth_map_map_auth /auth_map_map_frag_singleton. setoid_rewrite <- own_op.
     iApply (gen_own_update with "N").
     apply: auth_update_dfrac_alloc.
-    rewrite fmap_fmap_to_agree_singleton.
     eapply singleton_included_look.
-    { rewrite /fmap_fmap_to_agree lookup_fmap mLook /=. reflexivity. }
-    simpl.
-    rewrite map_fmap_singleton.
-    eapply singleton_included_look.
-    { rewrite lookup_fmap. rewrite hLook. simpl. reflexivity. }
-    { done. }
+    { rewrite /agree_uncurry_map lookup_fmap lookup_gmap_uncurry mLook /= hLook. reflexivity. }
+    done.
   Qed.
 
-  Lemma auth_map_map_insert_top `{!LeibnizEquiv A} γ m ℓ hist :
+  Lemma insert_gmap_uncurry_None k1 k2 v m:
+    m !! k1 = None ->
+    gmap_uncurry (<[k1:={[k2 := v]}]> m) = <[ (k1, k2) := v ]> (gmap_uncurry m).
+  Proof.
+    intros look.
+    apply map_eq.
+    intros [ℓ t].
+    destruct (decide (ℓ = k1)) as [ <- | ]; destruct (decide (t = k2)) as [ <- |  ];
+      rewrite lookup_gmap_uncurry ?lookup_insert /=.
+    - rewrite lookup_singleton //.
+    - rewrite ?lookup_insert_ne; try congruence.
+      rewrite lookup_gmap_uncurry look //.
+    - rewrite ?lookup_insert_ne /=; try congruence.
+      rewrite lookup_gmap_uncurry //.
+    - rewrite ?lookup_insert_ne /=; try congruence.
+      rewrite lookup_gmap_uncurry //.
+  Qed.
+
+  Lemma insert_gmap_uncurry_Some k1 k2 v m h:
+    m !! k1 = Some h ->
+    gmap_uncurry (<[k1:=<[k2 := v]> h]> m) = <[ (k1, k2) := v ]> (gmap_uncurry m).
+  Proof.
+    intros look.
+    apply map_eq.
+    intros [ℓ t].
+    destruct (decide (ℓ = k1)) as [ <- | ]; destruct (decide (t = k2)) as [ <- |  ];
+      rewrite lookup_gmap_uncurry ?lookup_insert /=.
+    - rewrite lookup_insert //.
+    - rewrite ?lookup_insert_ne; try congruence.
+      rewrite lookup_gmap_uncurry look //.
+    - rewrite ?lookup_insert_ne /=; try congruence.
+      rewrite lookup_gmap_uncurry //.
+    - rewrite ?lookup_insert_ne /=; try congruence.
+      rewrite lookup_gmap_uncurry //.
+  Qed.
+
+  Lemma auth_map_map_insert_top `{!LeibnizEquiv A} γ m ℓ t a :
     m !! ℓ = None →
     auth_map_map_auth γ m ==∗
-    auth_map_map_auth γ (<[ℓ:=hist]> m) ∗
-    auth_map_map_frag γ {[ ℓ := hist ]}.
+    auth_map_map_auth γ (<[ℓ:= {[ t := a ]} ]> m) ∗
+    auth_map_map_frag_singleton γ ℓ t a.
   Proof.
     iIntros (look).
+    iIntros "(auth & #$ & #$)".
     rewrite -gen_own_op.
-    iApply @gen_own_update.
+    iApply (gen_own_update with "auth").
     apply auth_update_alloc.
-    rewrite /fmap_fmap_to_agree.
+    rewrite /agree_uncurry_map.
+    rewrite insert_gmap_uncurry_None; last done.
     rewrite fmap_insert.
-    rewrite map_fmap_singleton.
     apply alloc_local_update.
-    - rewrite lookup_fmap look. done.
-    - apply valid_to_agree_fmap.
+    - rewrite lookup_fmap lookup_gmap_uncurry look. done.
+    - done.
   Qed.
 
   (* NOTE: The requirement on leibniz equiv may not be strictly necessary, but
@@ -166,104 +117,92 @@ Section auth_map_map.
     h !! t = None →
     auth_map_map_auth γ m ==∗
     auth_map_map_auth γ (<[ℓ:=<[t:=a]> h]> m) ∗
-      auth_map_map_frag γ ({[ ℓ:=<[t:=a]> h ]}) ∗
-      auth_map_map_frag_singleton γ ℓ t a.
+    auth_map_map_frag_singleton γ ℓ t a.
   Proof.
-    iIntros (mLook hLook) "N".
-    iMod (gen_own_update _ _ (● fmap_fmap_to_agree (<[ℓ:=<[t:=a]> h]> m)) with "N ") as "H".
-    { apply auth_auth_grow.
-      { apply fmap_fmap_to_agree_valid. }
-      apply fmap_fmap_to_agree_incl.
-      * set_solver.
-      * intros ℓ' mi mi' look1 look2.
-        destruct (decide (ℓ = ℓ')).
-        + simplify_eq.
-          rewrite lookup_insert in look2.
-          simplify_eq.
-          by apply insert_subseteq.
-        + rewrite lookup_insert_ne in look2; last done.
-          simplify_eq.
-          reflexivity. }
-    rewrite assoc. rewrite comm.
-    iMod (gen_own_update with "H") as "[H $]".
-    { apply: auth_update_dfrac_alloc.
-      rewrite /fmap_fmap_to_agree.
-      rewrite -> fmap_insert.
-      rewrite map_fmap_singleton.
-      apply singleton_included_insert.
-      apply to_agree_fmap.
-      apply map_singleton_subseteq_l.
-      apply lookup_insert. }
-    iMod (gen_own_update with "H") as "[$ $]".
-    { apply: auth_update_dfrac_alloc.
-      rewrite /fmap_fmap_to_agree.
-      rewrite -> fmap_insert.
-      rewrite map_fmap_singleton.
-      apply singleton_included_insert.
-      apply to_agree_fmap.
-      reflexivity. }
-    done.
+    iIntros (look1 look2) "(auth & #$ & #$)".
+    rewrite -gen_own_op.
+    iApply (gen_own_update with "auth").
+    apply auth_update_alloc.
+    rewrite /agree_uncurry_map.
+    rewrite insert_gmap_uncurry_Some; last done.
+    rewrite fmap_insert.
+    apply alloc_local_update.
+    - rewrite lookup_fmap lookup_gmap_uncurry look1 /= look2. done.
+    - done.
   Qed.
 
-  Lemma auth_map_map_auth_frag `{!OfeDiscrete A} `{!LeibnizEquiv A} γ dq m ℓ t a :
-    auth_map_map_auth_dq γ dq m -∗
+  Lemma auth_map_map_auth_frag `{!OfeDiscrete A} `{!LeibnizEquiv A} γ m ℓ t a :
+    auth_map_map_auth γ m -∗
     auth_map_map_frag_singleton γ ℓ t a -∗
     ⌜ ∃ h, m !! ℓ = Some h ∧ h !! t = Some a ⌝.
   Proof.
-    iIntros "O F".
+    iIntros "[O _] [F _]".
+    iDestruct (gen_own_valid with "O") as %val.
+    rewrite auth_auth_valid in val.
     iDestruct (gen_own_valid_2 with "O F") as %V.
     iPureIntro.
     apply auth_both_dfrac_valid_discrete in V as (_ & incl & _).
-    apply fmap_fmap_to_agree_singleton_included_l in incl.
-    destruct incl as (h & equiv & sub).
-    exists h.
-    split. { apply leibniz_equiv. apply equiv. }
-    apply map_singleton_subseteq_l. done.
+    apply singleton_included_l in incl as (a' & look & sub%Some_included_total).
+    rewrite /agree_uncurry_map lookup_fmap lookup_gmap_uncurry in look.
+    rewrite ?Some_included_total in sub.
+    destruct (m !! ℓ) as [h | ]; simpl in look.
+    - exists h.
+      split; first done.
+      simpl in *.
+      apply fmap_Some_equiv in look as [v [look' equiv]].
+      rewrite equiv to_agree_included in sub.
+      apply leibniz_equiv in sub.
+      congruence.
+    - simpl in look.
+      symmetry in look.
+      apply None_equiv_eq in look.
+      congruence.
   Qed.
 
-  Lemma auth_map_map_frag_lookup `{!LeibnizEquiv A} γ m ℓ h :
-    m !! ℓ = Some h →
-    auth_map_map_frag γ m -∗
-    auth_map_map_frag γ {[ ℓ := h ]}.
-  Proof.
-    iIntros (mLook).
-    rewrite /auth_map_map_frag.
-    rewrite /auth_map_map_frag_singleton.
-    rewrite /auth_map_map_frag.
-    iApply @gen_own_mono.
-    simpl.
-    apply auth_frag_mono.
-    rewrite /fmap_fmap_to_agree.
-    rewrite map_fmap_singleton.
-    apply singleton_included_l.
-    eexists _.
-    split. { rewrite lookup_fmap. rewrite mLook. simpl. reflexivity. }
-    done.
-  Qed.
+  (* Lemma auth_map_map_frag_lookup `{!LeibnizEquiv A} γ m ℓ h : *)
+  (*   m !! ℓ = Some h → *)
+  (*   auth_map_map_frag γ m -∗ *)
+  (*   auth_map_map_frag γ {[ ℓ := h ]}. *)
+  (* Proof. *)
+  (*   iIntros (mLook). *)
+  (*   rewrite /auth_map_map_frag. *)
+  (*   rewrite /auth_map_map_frag_singleton. *)
+  (*   rewrite /auth_map_map_frag. *)
+  (*   iIntros "(F & $ & $)". *)
+  (*   iApply (gen_own_mono with "F"). *)
+  (*   simpl. *)
+  (*   apply auth_frag_mono. *)
+  (*   rewrite /fmap_fmap_to_agree. *)
+  (*   rewrite map_fmap_singleton. *)
+  (*   apply singleton_included_l. *)
+  (*   eexists _. *)
+  (*   split. { rewrite lookup_fmap. rewrite mLook. simpl. reflexivity. } *)
+  (*   done. *)
+  (* Qed. *)
 
-  Lemma auth_map_map_frag_lookup_singleton `{!LeibnizEquiv A} γ m ℓ h t a :
-    m !! ℓ = Some h →
-    h !! t = Some a →
-    auth_map_map_frag γ m -∗
-    auth_map_map_frag_singleton γ ℓ t a.
-  Proof.
-    iIntros (mLook hLook).
-    rewrite /auth_map_map_frag.
-    rewrite /auth_map_map_frag_singleton.
-    rewrite /auth_map_map_frag.
-    iApply @gen_own_mono.
-    simpl.
-    apply auth_frag_mono.
-    rewrite /fmap_fmap_to_agree.
-    rewrite map_fmap_singleton.
-    apply singleton_included_l.
-    eexists _.
-    split. { rewrite lookup_fmap. rewrite mLook. simpl. reflexivity. }
-    apply Some_included_total.
-    apply to_agree_fmap.
-    apply map_singleton_subseteq_l.
-    done.
-  Qed.
+  (* Lemma auth_map_map_frag_lookup_singleton `{!LeibnizEquiv A} γ m ℓ h t a : *)
+  (*   m !! ℓ = Some h → *)
+  (*   h !! t = Some a → *)
+  (*   auth_map_map_frag γ m -∗ *)
+  (*   auth_map_map_frag_singleton γ ℓ t a. *)
+  (* Proof. *)
+  (*   iIntros (mLook hLook) "(F & #$ & #$)". *)
+  (*   rewrite /auth_map_map_frag. *)
+  (*   rewrite /auth_map_map_frag_singleton. *)
+  (*   rewrite /auth_map_map_frag. *)
+  (*   iApply (gen_own_mono with "F"). *)
+  (*   simpl. *)
+  (*   apply auth_frag_mono. *)
+  (*   rewrite /fmap_fmap_to_agree. *)
+  (*   rewrite map_fmap_singleton. *)
+  (*   apply singleton_included_l. *)
+  (*   eexists _. *)
+  (*   split. { rewrite lookup_fmap. rewrite mLook. simpl. reflexivity. } *)
+  (*   apply Some_included_total. *)
+  (*   apply to_agree_fmap. *)
+  (*   apply map_singleton_subseteq_l. *)
+  (*   done. *)
+  (* Qed. *)
 
   Lemma auth_map_map_lookup_agree `{!OfeDiscrete A} `{!LeibnizEquiv A} γ m ℓ h t a a' :
     m !! ℓ = Some h →
@@ -272,11 +211,80 @@ Section auth_map_map.
     auth_map_map_frag_singleton γ ℓ t a' -∗
     ⌜ a = a' ⌝.
   Proof.
-    iIntros (mLook hLook) "O F".
-    iDestruct (auth_map_map_auth_frag with "O F") as %(? & ? & ?).
+    iIntros (mLook hLook) "[O _] [F _]".
+    iDestruct (gen_own_valid_2 with "O F") as %[(? & look & incl)%singleton_included_l _]%auth_both_valid_discrete.
+    rewrite /agree_uncurry_map lookup_fmap lookup_gmap_uncurry in look.
+    rewrite ?Some_included_total in incl.
+    rewrite mLook /= hLook in look.
+    apply fmap_Some_equiv in look as [v [look' equiv]].
+    rewrite equiv to_agree_included in incl.
+    apply leibniz_equiv in incl.
     iPureIntro. congruence.
   Qed.
-
 End auth_map_map.
+Notation auth_map_mapR_inG A Σ Ω := (genInDepsG Σ Ω (auth_map_mapR A) [#crashed_atR]).
 
-Notation auth_map_mapR_inG Σ Ω A := (genInDepsG Σ Ω (auth_map_mapR A) [#crashed_atR]).
+Section history.
+  Implicit Types (histories: gmap loc (gmap time message)).
+  Context `{!nvmBaseGS Σ Ω, inG: !auth_map_mapR_inG (leibnizO message) Σ Ω}.
+  
+  Definition drop_above_map_uncurry (OCV: view.view):
+    (auth_map_mapR (leibnizO message) → auth_map_mapR (leibnizO message)) :=
+    fmap_auth (map_imap (λ '(ℓ, t) a, if decide (ℓ ∈ dom OCV ∧ t ≤ OCV !!0 ℓ) then Some $ agree_map discard_msg_views a else None)).
+
+  Definition histories_rel: rel_over [#crashed_atR] (auth_map_mapR (leibnizO message)) :=
+    λ tC tH, ∃ OCV,
+      tC = crashed_at_trans OCV ∧
+      tH = drop_above_map_uncurry OCV.
+
+  #[global] Instance own_all_phys_histories_nextgen γ histories:
+    IntoNextgen
+      (auth_map_map_auth histories_rel γ histories)
+      (∀ OCV, crashed_at_offset OCV -∗
+              auth_map_map_auth histories_rel γ (drop_above_map OCV histories)).
+  Proof.
+    rewrite /IntoNextgen.
+    iNamed 1.
+    iModIntro.
+    iDestruct "crashed" as (OV OCV' tC) "[pickedC crashed]".
+    iDestruct "rely" as "[rely (%tH & %tC' & [% _] & pickedH & pickedC')]".
+    iDestruct "own_auth" as (tH') "[#pickedH' own_auth]".
+    iPickedInAgree "pickedC pickedC'".
+    iPickedInAgree "pickedH pickedH'".
+    destruct H as (OCV'' & -> & ->).
+    iIntros (?) "offset".
+    simpl.
+    iAssert ⌜ OCV = OCV'' ⌝%I as %<-.
+    { iNamed "offset".
+      iDestruct (crashed_at_both_agree with "offset crashed") as %[-> ->].
+      done. }
+    rewrite /auth_map_map_auth.
+    iFrame "rely".
+    iSplit; last by iExists _, _.
+    iApply (gen_own_mono with "own_auth").
+    rewrite /drop_above_map_uncurry fmap_auth_auth.
+    rewrite auth_auth_included.
+    rewrite map_equiv_iff.
+    intros [ℓ t].
+    rewrite /agree_uncurry_map /drop_above_map map_lookup_imap ?lookup_fmap ?lookup_gmap_uncurry /= map_lookup_imap /=.
+    destruct (histories !! ℓ) as [h | ] eqn:Heq1; rewrite ?Heq1 /=; last done.
+    rewrite /drop_above_hist.
+    destruct (OCV !! ℓ) as [[tC] | ] eqn:Heqn2; rewrite ?Heqn2 /=.
+    - rewrite lookup_fmap.
+      destruct (decide (t ≤ tC)).
+      + rewrite map_extra.drop_above_lookup_le; last done.
+        destruct (h !! t) eqn:Heqn3; rewrite ?Heqn3 /=; last done.
+        rewrite decide_True ?agree_map_to_agree //.
+        split; first by eapply elem_of_dom_2.
+        rewrite /lookup_zero Heqn2 /= //.
+      + rewrite map_extra.drop_above_lookup_gt; last lia.
+        destruct (h !! t) eqn:Heqn3; rewrite ?Heqn3 /=; last done.
+        rewrite decide_False //.
+        rewrite /lookup_zero Heqn2 /=.
+        lia.
+    - destruct (h !! t) eqn:Heqn3; rewrite ?Heqn3 /=; last done.
+      rewrite decide_False //.
+      rewrite -not_elem_of_dom in Heqn2.
+      set_solver.
+  Qed.
+End history.
